thys/Jeroslow.thy
@@ -1,17 +1,18 @@
 theory Jeroslow imports 
-Abstract_Representability Diagonalization
+Abstract_Representability Diagonalization PseudoTerms
 begin 
 
 (* The Jeroslow assumptions: *)
 (*****************************)
 
 locale Jeroslow_Diagonalization = 
-Deduct2_with_False 
+Deduct_with_False_Disj_Rename
   var trm fmla Var FvarsT substT Fvars subst
   eql cnj imp all exi 
   fls
+  dsj
   num
-  prv prv
+  prv 
 +
 Encode
   var trm fmla Var FvarsT substT Fvars subst
@@ -19,102 +20,130 @@ Encode
   eql cnj imp all exi 
   prv prv
   enc 
-+
+(* +
 TermEncode
   var trm fmla Var FvarsT substT Fvars subst
   num
   eql cnj imp all exi 
   prv prv
-  Ops tenc  
+  Ops tenc  *)
 for 
 var :: "'var set" and trm :: "'trm set" and fmla :: "'fmla set" 
 and Var FvarsT substT Fvars subst  
 and eql cnj imp all exi 
 and fls 
+and dsj
 and num
 and prv 
-and enc ("\<langle>_\<rangle>") 
-and Ops and tenc  
-+  
+and enc ("\<langle>_\<rangle>")  
++   
 fixes F :: "('trm \<Rightarrow> 'trm) set"
-  and encF :: "('trm \<Rightarrow> 'trm) \<Rightarrow> ('trm \<Rightarrow> 'trm)" 
+  and encF :: "('trm \<Rightarrow> 'trm) \<Rightarrow> 'fmla" 
   and N :: "'trm \<Rightarrow> 'trm"
   and ssap :: "'fmla \<Rightarrow> 'trm \<Rightarrow> 'trm"  
 (*  *)
 assumes 
+(* For the members f of F, we only care about their action on numerals: *)
 F[simp,intro!]: "\<And> f n. f \<in> F \<Longrightarrow> n \<in> num \<Longrightarrow> f n \<in> num"
 and
-encF[simp,intro!]: "\<And> f. f \<in> F \<Longrightarrow> encF f \<in> Ops"
+encF[simp,intro!]: "\<And> f. f \<in> F \<Longrightarrow> encF f \<in> ptrm (Suc 0)"
 and 
 N[simp,intro!]: "N \<in> F" 
 and 
-ssap[simp]: "\<And>\<phi>. \<phi> \<in> fmla \<Longrightarrow> Fvars \<phi> = {xx} \<Longrightarrow> ssap \<phi> \<in> F"
+ssap[simp]: "\<And>\<phi>. \<phi> \<in> fmla \<Longrightarrow> Fvars \<phi> = {inp} \<Longrightarrow> ssap \<phi> \<in> F"
 (*  *)
 and 
-ReprF: "\<And>f n. f \<in> F \<Longrightarrow> n \<in> num \<Longrightarrow> prv (eql (encF f n) (f n))"
+ReprF: "\<And>f n. f \<in> F \<Longrightarrow> n \<in> num \<Longrightarrow> prveqlPT (instInp (encF f) n) (f n)"
 and
 CapN: "\<And>\<phi>. \<phi> \<in> fmla \<Longrightarrow> Fvars \<phi> = {} \<Longrightarrow> N \<langle>\<phi>\<rangle> = \<langle>neg \<phi>\<rangle>"
 and  
-CapSS: 
-"\<And> \<psi> f. \<psi> \<in> fmla \<Longrightarrow> Fvars \<psi> = {xx} \<Longrightarrow> f \<in> F \<Longrightarrow> 
-    ssap \<psi> (tenc (encF f)) = \<langle>inst \<psi> (encF f (tenc (encF f)))\<rangle>"
+CapSS: (* We consider formulas \<psi> of one variable, called "inp": *)
+"\<And> \<psi> f. \<psi> \<in> fmla \<Longrightarrow> Fvars \<psi> = {inp} \<Longrightarrow> f \<in> F \<Longrightarrow> 
+    ssap \<psi> \<langle>encF f\<rangle> = \<langle>cmpP \<psi> 0 (instInp (encF f) \<langle>encF f\<rangle>)\<rangle>" 
 begin 
 
-definition tJ :: "'fmla \<Rightarrow> 'trm" where 
-"tJ \<psi> \<equiv> encF (ssap \<psi>) (tenc (encF (ssap \<psi>)))"
+lemma encF_fmla[simp,intro!]: "\<And> f. f \<in> F \<Longrightarrow> encF f \<in> fmla"
+by auto
+
+lemma enc_trm: "\<phi> \<in> fmla \<Longrightarrow> \<langle>\<phi>\<rangle> \<in> trm"
+by auto
+  
+
+definition \<tau>J :: "'fmla \<Rightarrow> 'fmla" where 
+"\<tau>J \<psi> \<equiv> instInp (encF (ssap \<psi>)) (\<langle>encF (ssap \<psi>)\<rangle>)"
 
 definition \<phi>J :: "'fmla \<Rightarrow> 'fmla" where 
-"\<phi>J \<psi> \<equiv> subst \<psi> (tJ \<psi>) xx" 
+"\<phi>J \<psi> \<equiv> cmpP \<psi> 0 (\<tau>J \<psi>)" 
 
-lemma tJ[simp]: 
-assumes "\<psi> \<in> fmla" and "Fvars \<psi> = {xx}"
-shows "tJ \<psi> \<in> trm"
-using assms tJ_def by auto
+lemma \<tau>J[simp]: 
+assumes "\<psi> \<in> fmla" and "Fvars \<psi> = {inp}"
+shows "\<tau>J \<psi> \<in> ptrm 0"
+unfolding \<tau>J_def apply(rule instInp)
+using assms by auto
 
-lemma FvarsT_tJ[simp]: 
-assumes "\<psi> \<in> fmla" and "Fvars \<psi> = {xx}"
-shows "FvarsT (tJ \<psi>) = {}"
-using assms tJ_def by auto
+lemma \<tau>J_fmla[simp]: 
+assumes "\<psi> \<in> fmla" and "Fvars \<psi> = {inp}"
+shows "\<tau>J \<psi> \<in> fmla"
+using \<tau>J[OF assms] unfolding ptrm_def by auto
+
+lemma FvarsT_\<tau>J[simp]: 
+assumes "\<psi> \<in> fmla" and "Fvars \<psi> = {inp}"
+shows "Fvars (\<tau>J \<psi>) = {out}"
+using \<tau>J[OF assms] unfolding ptrm_def by auto
 
 lemma \<phi>J[simp]: 
-assumes "\<psi> \<in> fmla" and "Fvars \<psi> = {xx}"
+assumes "\<psi> \<in> fmla" and "Fvars \<psi> = {inp}"
 shows "\<phi>J \<psi> \<in> fmla"
-using assms \<phi>J_def by auto
+unfolding \<phi>J_def apply(rule cmpP_fmla)
+using assms by auto
 
 lemma Fvars_\<phi>J[simp]: 
-assumes "\<psi> \<in> fmla" and "Fvars \<psi> = {xx}"
+assumes "\<psi> \<in> fmla" and "Fvars \<psi> = {inp}"
 shows "Fvars (\<phi>J \<psi>) = {}"
-using assms \<phi>J_def by (auto simp: Fvars_subst)
+using assms unfolding \<phi>J_def by (auto simp: Fvars_cmpP2)
 
 lemma diagonalization: 
-assumes "\<psi> \<in> fmla" and "Fvars \<psi> = {xx}"
-shows "prv (eql (tJ \<psi>) \<langle>inst \<psi> (tJ \<psi>)\<rangle>) \<and> 
-       prv (eqv (\<phi>J \<psi>) (inst \<psi> \<langle>\<phi>J \<psi>\<rangle>))"
+assumes \<psi>[simp]: "\<psi> \<in> fmla" and [simp]: "Fvars \<psi> = {inp}"
+shows "prveqlPT (\<tau>J \<psi>) \<langle>cmpP \<psi> 0 (\<tau>J \<psi>)\<rangle> \<and> 
+       prv (eqv (\<phi>J \<psi>) (instInp \<psi> \<langle>\<phi>J \<psi>\<rangle>))"
 proof 
-  define fJ where "fJ \<equiv> ssap \<psi>" 
-  have fJ[simp]: "fJ \<in> F" unfolding fJ_def using assms by auto
-  have "fJ (tenc (encF fJ)) = \<langle>inst \<psi> (tJ \<psi>)\<rangle>"
-   by (simp add: CapSS assms fJ_def tJ_def)
-  thus **: "prv (eql (tJ \<psi>) \<langle>inst \<psi> (tJ \<psi>)\<rangle>)"   
-   using ReprF fJ fJ_def tJ_def by fastforce
-  show "prv (eqv (\<phi>J \<psi>) (inst \<psi> \<langle>\<phi>J \<psi>\<rangle>))"
-   using assms prv_eql_subst_trm_eqv[OF xx _  _ _ **, of "\<psi>"] 
-   by (auto simp: \<phi>J_def inst_def) 
+  define f where "f \<equiv> ssap \<psi>" 
+  have f[simp]: "f \<in> F" unfolding f_def using assms by auto
+  have ff: "f \<langle>encF f\<rangle> = \<langle>cmpP \<psi> 0 (\<tau>J \<psi>)\<rangle>"
+  using assms unfolding f_def \<tau>J_def by (intro CapSS) auto
+
+  show "prveqlPT (\<tau>J \<psi>) \<langle>cmpP \<psi> 0 (\<tau>J \<psi>)\<rangle>" 
+  using ReprF[OF f, of "\<langle>encF f\<rangle>"]  
+  unfolding \<tau>J_def[of \<psi>, unfolded f_def[symmetric],symmetric] ff[symmetric]
+  by auto 
+  from prveqlPT_prv_instInp_eqv_cmpP[OF \<psi>, of "\<tau>J \<psi>", OF _ _ _ _ this,
+           unfolded \<phi>J_def[symmetric]]
+  show "prv (eqv (\<phi>J \<psi>) (instInp \<psi> \<langle>\<phi>J \<psi>\<rangle>))"
+  by auto  
 qed 
 
 
 end \<comment> \<open>context Jeroslow_Diagonalization\<close>
 
+context WRepr_Provability 
+begin
+
+(* Changing the variable (from xx to inp) in the provability predicate: *)
+definition "Pinp \<equiv> subst P (Var inp) xx"
+lemma PP_Pinp: "t \<in> trm \<Longrightarrow> PP t = instInp Pinp t"
+unfolding PP_def Pinp_def instInp_def by auto
+
+end (* context WRepr_Provability  *)
 
 locale Jeroslow_Godel_Second =  
 Jeroslow_Diagonalization 
   var trm fmla Var FvarsT substT Fvars subst
   eql cnj imp all exi 
   fls
+  dsj
   num
   prv 
   enc    
-  Ops tenc 
   F encF N ssap
 +
 WRepr_Provability
@@ -129,23 +158,26 @@ var :: "'var set" and trm :: "'trm set" and fmla :: "'fmla set"
 and Var FvarsT substT Fvars subst  
 and eql cnj imp all exi 
 and fls 
+and dsj
 and num
 and prv 
-and enc ("\<langle>_\<rangle>") 
-and Ops and tenc 
+and enc ("\<langle>_\<rangle>")  
 and P
 and F encF N ssap
 + 
-assumes 
-HBL1: "\<And>\<phi>. \<phi> \<in> fmla \<Longrightarrow> Fvars \<phi> = {} \<Longrightarrow> prv \<phi> \<Longrightarrow> prv (PP \<langle>\<phi>\<rangle>)" 
-and 
-SHBL3: "\<And>t. t \<in> trm \<Longrightarrow> FvarsT t = {} \<Longrightarrow> prv (imp (PP t) (PP \<langle>PP t\<rangle>))"
+assumes  
+SHBL3: "\<And>\<tau>. \<tau> \<in> ptrm 0 \<Longrightarrow> prv (imp (cmpP Pinp 0 \<tau>) (instInp Pinp \<langle>cmpP Pinp 0 \<tau>\<rangle>))"
 begin
 
+(* A version of HBL1 that uses the inp variable: *)
+lemma HBL1_inp: 
+"\<phi> \<in> fmla \<Longrightarrow> Fvars \<phi> = {} \<Longrightarrow> prv \<phi> \<Longrightarrow> prv (instInp Pinp \<langle>\<phi>\<rangle>)"
+unfolding Pinp_def instInp_def by (auto intro: HBL1)
   
 (* Consistency formula a la Jeroslow: *)
 definition jcons :: "'fmla" where 
-"jcons \<equiv> all xx (neg (cnj (PP (Var xx)) (PP (encF N (Var (xx))))))" 
+"jcons \<equiv> all xx (neg (cnj (instInp Pinp (Var xx)) 
+                           (cmpP Pinp 0 (instInp (encF N) (Var (xx))))))" 
 
 lemma prv_eql_subst_trm3:
 "x \<in> var \<Longrightarrow> \<phi> \<in> fmla \<Longrightarrow> t1 \<in> trm \<Longrightarrow> t2 \<in> trm \<Longrightarrow> 
@@ -153,142 +185,142 @@ prv (eql t1 t2) \<Longrightarrow> prv (subst \<phi> t1 x) \<Longrightarrow> prv 
 using prv_eql_subst_trm2  
   by (meson subst prv_imp_mp) 
 
-lemma prv_eql_neg_encF_N: 
-assumes "\<phi> \<in> fmla" and "Fvars \<phi> = {}"
-shows "prv (eql \<langle>neg \<phi>\<rangle> (encF N \<langle>\<phi>\<rangle>))" 
-  unfolding CapN[symmetric, OF assms]
-  by (rule prv_prv_eql_sym) (auto simp: assms intro: ReprF)  
-  
-lemma prv_imp_neg_encF_N_aux: 
-assumes "\<phi> \<in> fmla" and "Fvars \<phi> = {}"
-shows "prv (imp (PP \<langle>neg \<phi>\<rangle>) (PP (encF N \<langle>\<phi>\<rangle>)))" 
-using assms prv_eql_subst_trm2[OF _ _ _ _ prv_eql_neg_encF_N[OF assms], 
-  of xx "PP (Var xx)"]  
-  unfolding PP_def by auto
+lemma Pinp[simp,intro!]: "Pinp \<in> fmla" 
+and Fvars_Pinp[simp]: "Fvars Pinp = {inp}"
+unfolding Pinp_def by (auto simp: Fvars_subst)
 
-
-lemma prv_cnj_neg_encF_N_aux: 
-assumes "\<phi> \<in> fmla" and "Fvars \<phi> = {}" "\<chi> \<in> fmla" "Fvars \<chi> = {}"
-and "prv (neg (cnj \<chi> (PP \<langle>neg \<phi>\<rangle>)))"
-shows"prv (neg (cnj \<chi> (PP (encF N \<langle>\<phi>\<rangle>))))"
-using assms prv_eql_subst_trm3[OF _ _ _ _ prv_eql_neg_encF_N, 
-  of xx "neg (cnj \<chi> (PP (Var xx)))"] 
-  unfolding PP_def by auto
+lemma ReprF_combineWith_CapN: 
+assumes "\<phi> \<in> fmla" and "Fvars \<phi> = {}"
+shows "prveqlPT (instInp (encF N) \<langle>\<phi>\<rangle>) \<langle>neg \<phi>\<rangle>" 
+using assms unfolding CapN[symmetric, OF assms] by (intro ReprF) auto  
  
 theorem jeroslow_godel_second: 
 assumes consistent
+(* Implicit unreasonable assumption under which Jeroslow's formulation works: *)
+assumes unreasonable:
+        "let \<psi> = cmpP Pinp (Suc 0) (encF N); 
+             \<tau> = \<tau>J \<psi>; 
+             \<phi> = cmpP (cmpP Pinp (Suc 0) (encF N)) 0 \<tau>;  
+             \<phi>' = cmpP Pinp 0 (cmpP (encF N) 0 \<tau>) 
+         in prv (eql \<langle>\<phi>\<rangle> \<langle>\<phi>'\<rangle>)"
 shows "\<not> prv jcons"
-proof
+proof 
   assume *: "prv jcons"
-  define \<psi> where "\<psi> \<equiv> PP (encF N (Var xx))"
-  define t where "t \<equiv> tJ \<psi>"
-  have \<psi>[simp,intro]: "\<psi> \<in> fmla" "Fvars \<psi> = {xx}" 
-  and t[simp,intro]: "t \<in> trm" "FvarsT t = {}" 
-    unfolding \<psi>_def t_def by auto
 
-  have sPP[simp]: "subst (PP (encF N (Var xx))) \<langle>PP (encF N t)\<rangle> xx = 
-             PP (encF N \<langle>PP (encF N t)\<rangle>)"
-    unfolding PP_def by (subst subst_compose_eq_or) auto
-  have sPP2[simp]: "subst (PP (encF N (Var xx))) t xx = PP (encF N t)"
-    unfolding PP_def by (subst subst_compose_eq_or) auto
-  have 00: "PP (encF N t) = inst \<psi> t" unfolding \<psi>_def inst_def PP_def
-    by (subst subst_compose_eq_or) auto
-  
+  define \<psi> where "\<psi> \<equiv> cmpP Pinp (Suc 0) (encF N)"
+  define \<tau> where "\<tau> \<equiv> \<tau>J \<psi>"
   define \<phi> where "\<phi> \<equiv> \<phi>J \<psi>"
+  have \<psi>[simp,intro]: "\<psi> \<in> fmla" "Fvars \<psi> = {inp}" 
+  unfolding \<psi>_def by (auto simp: Fvars_cmpP2) 
+  have \<tau>[simp,intro]: "\<tau> \<in> ptrm 0" "\<tau> \<in> fmla" "Fvars \<tau> = {out}" 
+    unfolding \<tau>_def by auto
   have [simp]: "\<phi> \<in> fmla" "Fvars \<phi> = {}" unfolding \<phi>_def by auto
-  have **: "prv (eql t \<langle>\<phi>\<rangle>)" 
-    unfolding 00 \<phi>_def 
-    using \<phi>J_def diagonalization inst_def t_def by auto
-  have \<phi>: "\<phi> = PP (encF N t)" unfolding \<phi>_def \<phi>J_def t_def \<psi>_def 
-    using sPP2 \<psi>_def t_def by blast
-  have 1: "prv (imp \<phi> (PP \<langle>\<phi>\<rangle>))" using SHBL3[of "encF N t"] 
-    using 00 \<phi>J_def \<phi>_def \<psi>_def inst_def t_def by auto
-  have eqv_\<phi>: "prv (eqv \<phi> (PP (encF N \<langle>\<phi>\<rangle>)))"  using diagonalization
-    by (metis "00" sPP \<phi>J_def \<phi>_def \<psi> \<psi>_def diagonalization inst_def t_def)
-  have 2: "prv (imp \<phi> (PP (encF N \<langle>\<phi>\<rangle>)))" 
-   using prv_cnjEL[OF _ _ eqv_\<phi>[unfolded eqv_def]] by auto 
-  have "prv (imp (PP (encF N \<langle>\<phi>\<rangle>)) \<phi>)"
-   using prv_cnjER[OF _ _ eqv_\<phi>[unfolded eqv_def]] by auto 
-  from  prv_prv_imp_trans[OF _ _ _ prv_imp_neg_encF_N_aux this]
-  have 22: "prv (imp (PP \<langle>neg \<phi>\<rangle>) \<phi>)" by auto
-  have 3: "prv (imp \<phi> (cnj (PP \<langle>\<phi>\<rangle>) (PP (encF N \<langle>\<phi>\<rangle>))))" 
-    by (rule prv_imp_cnj[OF _ _ _ 1 2]) (auto simp: \<phi>_def)
-  have 4: "prv (neg (cnj (PP \<langle>\<phi>\<rangle>) (PP (encF N \<langle>\<phi>\<rangle>))))" 
-     using prv_allE[OF _ _ _ *[unfolded jcons_def], of "\<langle>\<phi>\<rangle>"] 
-  by (simp add: \<phi> \<psi>_def)
-  have 5: "prv (neg \<phi>)" 
-    unfolding neg_def 
-    by (rule prv_prv_imp_trans[OF _ _ _ 3 4[unfolded neg_def]]) auto
-  hence "prv (PP \<langle>neg \<phi>\<rangle>)" using  
-      HBL1[OF _ _ 5] by auto
-  hence "prv \<phi>" using prv_imp_mp[OF _ _ 22] by auto
-  with 5 assms show False unfolding consistent_def3 by auto
-qed
+
+  define eN\<tau> where "eN\<tau> \<equiv> cmpP (encF N) 0 \<tau>"
+  have eN\<tau>[simp]: "eN\<tau> \<in> ptrm 0" "eN\<tau> \<in> fmla" "Fvars eN\<tau> = {out}"
+   unfolding eN\<tau>_def by (auto simp: cmpP1 Fvars_cmpP)
+  define \<phi>' where "\<phi>' \<equiv> cmpP Pinp 0 eN\<tau>" 
+  have [simp]: "\<phi>' \<in> fmla" "Fvars \<phi>' = {}" unfolding \<phi>'_def by (auto simp: Fvars_cmpP)
+
+  have \<phi>\<phi>': "prv (imp \<phi> \<phi>')" and \<phi>'\<phi>: "prv (imp \<phi>' \<phi>)" and \<phi>e\<phi>': "prv (eqv \<phi> \<phi>')"
+   unfolding \<phi>_def \<phi>J_def \<phi>'_def eN\<tau>_def \<tau>_def[symmetric] unfolding \<psi>_def
+   using prv_cmpP_compose[of Pinp "encF N" \<tau>] by auto
+
+  from diagonalization[OF \<psi>]
+  have "prveqlPT \<tau> \<langle>cmpP \<psi> 0 \<tau>\<rangle>" and **: "prv (eqv \<phi> (instInp \<psi> \<langle>\<phi>\<rangle>))" 
+  unfolding \<tau>_def[symmetric] \<phi>_def[symmetric] by auto
+  have "**1": "prv (imp \<phi> (instInp \<psi> \<langle>\<phi>\<rangle>))" "prv (imp (instInp \<psi> \<langle>\<phi>\<rangle>) \<phi>)"
+   using prv_imp_eqvEL[OF _ _ **] prv_imp_eqvER[OF _ _ **] by auto
+
+  from SHBL3[OF eN\<tau>(1)] 
+  have "prv (imp (cmpP Pinp 0 eN\<tau>) (instInp Pinp \<langle>cmpP Pinp 0 eN\<tau>\<rangle>))" .
+  hence "prv (imp \<phi>' (instInp Pinp \<langle>\<phi>'\<rangle>))" unfolding \<phi>'_def .
+  from prv_prv_imp_trans[OF _ _ _ \<phi>\<phi>' this]
+  have 0: "prv (imp \<phi> (instInp Pinp \<langle>\<phi>'\<rangle>))" by auto
+
+  note unr = unreasonable[unfolded Let_def 
+    \<phi>_def[unfolded \<phi>J_def \<tau>_def[symmetric], symmetric] \<psi>_def[symmetric] 
+      \<tau>_def[symmetric] eN\<tau>_def[symmetric] \<phi>'_def[symmetric] \<phi>J_def] 
+
+  have 1: "prv (imp \<phi> (instInp Pinp \<langle>\<phi>\<rangle>))"
+  apply(rule nprv_prvI, auto)
+  apply(rule nprv_impI, auto)
+  apply(rule nprv_addLemmaE[OF unr], auto)
+  apply(rule nprv_addImpLemmaE[OF 0], auto intro: nprv_hyp)
+  apply(rule nprv_clear3_3, auto)
+  apply(rule nprv_eql_substE01[of "\<langle>\<phi>\<rangle>" "\<langle>\<phi>'\<rangle>" _ "instInp Pinp (Var xx)" xx], 
+     auto simp: instInp_def nprv_hyp) . 
+
+  have 2: "prv (imp \<phi> (cnj (instInp Pinp \<langle>\<phi>\<rangle>) 
+                           (instInp \<psi> \<langle>\<phi>\<rangle>)))"
+  apply(rule nprv_prvI, auto)
+  apply(rule nprv_impI, auto)
+  apply(rule nprv_cnjI, auto)
+  subgoal apply(rule nprv_addImpLemmaE[OF 1], auto intro: nprv_hyp) .
+  subgoal apply(rule nprv_addImpLemmaE[OF "**1"(1)], auto intro: nprv_hyp) . .
+
+  define z where "z \<equiv> Variable (Suc (Suc 0))" 
+  have z_facts[simp]: "z \<in> var" "z \<noteq> xx" "z \<notin> Fvars Pinp"
+    "out \<noteq> z \<and> z \<noteq> out" "inp \<noteq> z \<and> z \<noteq> inp" 
+   unfolding z_def by auto
+  have 30: "subst (cmpP Pinp 0 (instInp (encF N) (Var xx))) \<langle>\<phi>\<rangle> xx = 
+            cmpP Pinp 0 (instInp (encF N) \<langle>\<phi>\<rangle>)" 
+  unfolding z_def[symmetric] instInp_def cmpP_def Let_def apply auto 
+  apply(subst subst_compose_diff, auto)
+  apply(subst subst_subst, auto simp: Fvars_subst)
+  apply(subst subst_notIn[of _ _ xx], auto simp: Fvars_subst)
+  apply(subst subst_compose_diff, auto) . 
+
+  have 31: "subst (instInp Pinp (Var xx)) \<langle>\<phi>\<rangle> xx = 
+            instInp Pinp \<langle>\<phi>\<rangle>" unfolding instInp_def by auto
+              
+
+  have 3: "prv (neg (cnj (instInp Pinp \<langle>\<phi>\<rangle>) 
+                         (instInp \<psi> \<langle>\<phi>\<rangle>)))"
+  apply(rule nprv_prvI, auto)
+  apply(rule nprv_addLemmaE[OF *, unfolded jcons_def], auto)
+  apply(rule nprv_allE0[of _ _ _ "\<langle>\<phi>\<rangle>"], auto  simp: 30 31)
+  apply(rule nprv_clear2_2, auto)
+  apply(rule nprv_negI, auto)
+  apply(rule nprv_negE0, auto)
+  apply(rule nprv_clear2_2, auto)
+  apply(rule nprv_cnjE0, auto)
+  apply(rule nprv_clear3_3, auto)
+  apply(rule nprv_cnjI, auto)
+  subgoal 
+    apply(auto intro: nprv_hyp) .
+  subgoal 
+    apply(rule nprv_clear2_1, auto)
+    apply(auto simp: nprv_hyp instInp_cmpP \<psi>_def) . .
+
+  have ***: "prv (neg \<phi>)"
+  apply(rule nprv_prvI, auto) 
+  apply(rule nprv_negI, auto) 
+  apply(rule nprv_addImpLemmaE[OF 2], auto simp: nprv_hyp)
+  apply(rule nprv_addLemmaE[OF 3], auto)
+  apply(rule nprv_negE0, auto simp: nprv_hyp) .
+
+  have 4: "prv (instInp Pinp \<langle>neg \<phi>\<rangle>)" using HBL1_inp[OF _ _ ***] by auto
+
+  have 5: "prveqlPT (instInp (encF N) \<langle>\<phi>\<rangle>) \<langle>neg \<phi>\<rangle>"
+    using ReprF_combineWith_CapN[of \<phi>] by auto
+
+  have 6: "prv (cmpP Pinp 0 (instInp (encF N) \<langle>\<phi>\<rangle>))"
+  apply(rule nprv_prvI, auto)
+  apply(rule nprv_addLemmaE[OF 4], auto)
+  apply(rule prveqlPT_nprv_cmpP_instInp[OF _ _ _ _ _ 5], auto simp: instInp) .
+
+  note lem = "**1"(2)[unfolded \<psi>_def]
+  have "prv \<phi>"
+  apply(rule nprv_prvI, auto)
+  apply(rule nprv_addLemmaE[OF 6], auto)
+  apply(rule nprv_addImpLemmaE[OF lem], auto simp: nprv_hyp instInp_cmpP) .
+
+  from this *** `consistent` show False unfolding consistent_def3 by auto
+qed   
+   
  
-theorem jeroslow_godel_second_standardCon: 
-assumes consistent 
-and HBL4_prv: "\<And>\<phi>1 \<phi>2. {\<phi>1,\<phi>2} \<subseteq> fmla \<Longrightarrow> Fvars \<phi>1 = {} \<Longrightarrow> Fvars \<phi>2 = {} \<Longrightarrow> 
-   prv (imp (cnj (PP \<langle>\<phi>1\<rangle>) (PP \<langle>\<phi>2\<rangle>)) (PP \<langle>cnj \<phi>1 \<phi>2\<rangle>))"
-and WHBL2: "\<And>\<phi>1 \<phi>2. {\<phi>1,\<phi>2} \<subseteq> fmla \<Longrightarrow> Fvars \<phi>1 = {} \<Longrightarrow> Fvars \<phi>2 = {} \<Longrightarrow> 
-   prv (imp \<phi>1 \<phi>2) \<Longrightarrow> prv (imp (PP \<langle>\<phi>1\<rangle>) (PP \<langle>\<phi>2\<rangle>))"
-shows "\<not> prv (neg (PP \<langle>fls\<rangle>))"
-proof
-  assume *: (* jeroslow_godel_second's "prv jcons" is upgraded to: *) 
-    "prv (neg (PP \<langle>fls\<rangle>))"
-  define \<psi> where "\<psi> \<equiv> PP (encF N (Var xx))"
-  define t where "t \<equiv> tJ \<psi>"
-  have \<psi>[simp,intro]: "\<psi> \<in> fmla" "Fvars \<psi> = {xx}" 
-  and t[simp,intro]: "t \<in> trm" "FvarsT t = {}" 
-    unfolding \<psi>_def t_def by auto
-
-  have [simp]: "subst (PP (encF N (Var xx))) \<langle>PP (encF N t)\<rangle> xx = 
-             PP (encF N \<langle>PP (encF N t)\<rangle>)"
-    unfolding PP_def by (subst subst_compose_eq_or) auto
-  have [simp]: "subst (PP (encF N (Var xx))) t xx = PP (encF N t)"
-    unfolding PP_def by (subst subst_compose_eq_or) auto
-  have 00: "PP (encF N t) = inst \<psi> t" unfolding \<psi>_def inst_def PP_def
-    by (subst subst_compose_eq_or) auto
-  
-  define \<phi> where "\<phi> = PP (encF N t)"
-  have [simp]: "\<phi> \<in> fmla" "Fvars \<phi> = {}" unfolding \<phi>_def by auto
-  have **: "prv (eql t \<langle>PP (encF N t)\<rangle>)" 
-    unfolding 00 by (simp add: diagonalization t_def)
-  have 1: "prv (imp \<phi> (PP \<langle>\<phi>\<rangle>))" using SHBL3[of "encF N t"] 
-    by (auto simp: \<phi>_def)
-  have 2: "prv (imp \<phi> (PP (encF N \<langle>\<phi>\<rangle>)))"
-   using prv_eql_subst_trm2[OF xx _  _ _ **, of "PP (encF N (Var xx))"] 
-   by (auto simp: \<phi>_def)
-  have "prv (imp (PP (encF N \<langle>\<phi>\<rangle>)) \<phi>)"
-   using prv_eql_subst_trm_rev2[OF xx _  _ _ **, of "PP (encF N (Var xx))"] 
-   by (auto simp: \<phi>_def)
-  from prv_prv_imp_trans[OF _ _ _ prv_imp_neg_encF_N_aux this]
-  have 22: "prv (imp (PP \<langle>neg \<phi>\<rangle>) \<phi>)" by auto
-  have 3: "prv (imp \<phi> (cnj (PP \<langle>\<phi>\<rangle>) (PP (encF N \<langle>\<phi>\<rangle>))))" 
-    by (rule prv_imp_cnj[OF _ _ _ 1 2]) (auto simp: \<phi>_def)
-
-  (*  This is the modification from the proof of jeroslow_godel_second: *)
-  have 41: "prv (imp (cnj (PP \<langle>\<phi>\<rangle>) (PP \<langle>neg \<phi>\<rangle>)) (PP \<langle>cnj \<phi> (neg \<phi>)\<rangle>))"
-  using HBL4_prv[of \<phi> "neg \<phi>"] by auto
-  have "prv (imp (cnj \<phi> (neg \<phi>)) (fls))"  
-    by (simp add: prv_cnj_imp_monoR2 prv_imp_neg_fls)
-  from WHBL2[OF _ _ _ this] 
-  have 42: "prv (imp (PP \<langle>cnj \<phi> (neg \<phi>)\<rangle>) (PP \<langle>fls\<rangle>))" by auto
-  from prv_prv_imp_trans[OF _ _ _ 41 42]
-  have "prv (imp (cnj (PP \<langle>\<phi>\<rangle>) (PP \<langle>neg \<phi>\<rangle>)) (PP \<langle>fls\<rangle>))" by auto
-  from prv_prv_imp_trans[OF _ _ _ this *[unfolded neg_def]]
-  have "prv (neg (cnj (PP \<langle>\<phi>\<rangle>) (PP \<langle>neg \<phi>\<rangle>)))"
-  unfolding neg_def by auto
-  from prv_cnj_neg_encF_N_aux[OF _ _ _ _ this]
-  have 4: "prv (neg (cnj (PP \<langle>\<phi>\<rangle>) (PP (encF N \<langle>\<phi>\<rangle>))))" by auto
-  (*  End modification *)
-
-  have 5: "prv (neg \<phi>)" 
-    unfolding neg_def 
-    by (rule prv_prv_imp_trans[OF _ _ _ 3 4[unfolded neg_def]]) auto
-  hence "prv (PP \<langle>neg \<phi>\<rangle>)" using HBL1[OF _ _ 5] by auto
-  hence "prv \<phi>" using prv_imp_mp[OF _ _ 22] by auto
-  with 5 assms show False unfolding consistent_def3 by auto
-qed
+ 
 
 end \<comment> \<open>context Jeroslow_Godel_Second\<close>
 
