thys/Standard_Model.thy
@@ -84,27 +84,27 @@ and bprv
 and isTrue 
 +
 assumes 
-(* We assume soundness of the provability for sentences (w.r.t. truth): *)
-prv_sound_isTrue: 
+(* We assume Minimal_Truth_Soundness of the provability for sentences (w.r.t. truth): *)
+bprv_sound_isTrue: 
 "\<And>\<phi>. \<phi> \<in> fmla \<Longrightarrow> Fvars \<phi> = {} \<Longrightarrow> 
   bprv \<phi> \<Longrightarrow> isTrue \<phi>"
 begin
 
 (* For sound theories, consistency is a fact rather than a hypothesis *)
 lemma B_consistent: B.consistent
-  unfolding B.consistent_def using not_isTrue_fls prv_sound_isTrue by blast
+  unfolding B.consistent_def using not_isTrue_fls bprv_sound_isTrue by blast
 
 lemma prv_neg_excl:
 "\<phi> \<in> fmla \<Longrightarrow> Fvars \<phi> = {} \<Longrightarrow> 
   bprv \<phi> \<Longrightarrow> bprv (neg \<phi>) \<Longrightarrow> False"
-  using isTrue_neg_excl[of \<phi>] prv_sound_isTrue by auto
+  using isTrue_neg_excl[of \<phi>] bprv_sound_isTrue by auto
 
 lemma prv_imp_implies_isTrue: 
 assumes [simp,intro!]: "\<phi> \<in> fmla" "\<chi> \<in> fmla" "Fvars \<phi> = {}" "Fvars \<chi> = {}"
 and p: "bprv (imp \<phi> \<chi>)" and i: "isTrue \<phi>"
 shows "isTrue \<chi>" 
 proof-
-  have "isTrue (imp \<phi> \<chi>)" using p by (intro prv_sound_isTrue) auto
+  have "isTrue (imp \<phi> \<chi>)" using p by (intro bprv_sound_isTrue) auto
   thus ?thesis using assms isTrue_imp by blast
 qed
 
@@ -115,13 +115,13 @@ unfolding B.\<omega>consistent_def proof (safe del: notI)
   fix \<phi> x assume 0[simp,intro]: "\<phi> \<in> fmla"  "x \<in> var" and 1: "Fvars \<phi> = {x}"
   and 00: "\<forall>n\<in>num. bprv (neg (subst \<phi> n x))"
   hence "\<forall>n\<in>num. isTrue (neg (subst \<phi> n x))" 
-    using 00 1 by (auto intro!: prv_sound_isTrue simp: Fvars_subst)
+    using 00 1 by (auto intro!: bprv_sound_isTrue simp: Fvars_subst)
   hence "isTrue (all x (neg \<phi>))" by (simp add: "1" isTrue_all) 
   moreover 
   {have "bprv (imp (all x (neg \<phi>)) (neg (exi x \<phi>)))"  
     using B.prv_all_neg_imp_neg_exi by blast
    hence "isTrue (imp (all x (neg \<phi>)) (neg (exi x \<phi>)))"
-    by (simp add: "1" prv_sound_isTrue)
+    by (simp add: "1" bprv_sound_isTrue)
   }
   ultimately have "isTrue (neg (exi x \<phi>))"
     by (metis 0 1 Diff_insert_absorb Fvars_all Fvars_exi Fvars_neg all
@@ -129,7 +129,7 @@ unfolding B.\<omega>consistent_def proof (safe del: notI)
   hence "\<not> isTrue (neg (neg (exi x \<phi>)))"  
     using 1 isTrue_neg_excl by force 
   thus "\<not> bprv (neg (neg (exi x \<phi>)))"  
-    using "1" prv_sound_isTrue by auto 
+    using "1" bprv_sound_isTrue by auto 
 qed 
 
 lemma B_\<omega>consistentStd1: B.\<omega>consistentStd1
@@ -137,6 +137,7 @@ lemma B_\<omega>consistentStd1: B.\<omega>consistentStd1
 
 lemma B_\<omega>consistentStd2: B.\<omega>consistentStd2
   using B_\<omega>consistent B.\<omega>consistent_impliesStd2 by blast
+
 
 end 
 
@@ -188,7 +189,7 @@ lemma isTrue_prv_PPf_prf_or_neg:
   using not_prfOf_PPf prfOf_PPf by blast
 
 (* Hence that predicate is complete w.r.t. truth  *)
-lemma isTrue_implies_prv_PPf_prf: 
+lemma isTrue_PPf_Implies_bprv_PPf: 
 "prf \<in> proof \<Longrightarrow> \<phi> \<in> fmla \<Longrightarrow> Fvars \<phi> = {} \<Longrightarrow> 
    isTrue (PPf (encPf prf) \<langle>\<phi>\<rangle>) \<Longrightarrow> bprv (PPf (encPf prf) \<langle>\<phi>\<rangle>)"
   by (metis FvarsT_num Fvars_PPf Fvars_fls PPf 
@@ -197,30 +198,30 @@ neg_def not_isTrue_fls prv_imp_implies_isTrue)
 
 (* ... and thanks to cleanness we can replace encoded proofs 
 with arbitrary numerals in the completeness property:  *)
-lemma isTrue_implies_prv_PPf: 
+lemma isTrue_implies_bprv_PPf: 
 assumes [simp]: "n \<in> num" "\<phi> \<in> fmla" "Fvars \<phi> = {}" 
 and iT: "isTrue (PPf n \<langle>\<phi>\<rangle>)"
 shows "bprv (PPf n \<langle>\<phi>\<rangle>)" 
 proof(cases "n \<in> encPf ` proof")
   case True  
   thus ?thesis  
-    using iT isTrue_implies_prv_PPf_prf by auto  
+    using iT isTrue_PPf_Implies_bprv_PPf by auto  
 next
   case False
   hence "bprv (neg (PPf n \<langle>\<phi>\<rangle>))" by (simp add: PPf_encPf)
-  hence "isTrue (neg (PPf n \<langle>\<phi>\<rangle>))" by (intro prv_sound_isTrue) auto
+  hence "isTrue (neg (PPf n \<langle>\<phi>\<rangle>))" by (intro bprv_sound_isTrue) auto
   hence False using iT by (intro isTrue_neg_excl) auto
   thus ?thesis by auto
 qed
 
-(* In fact, by soundness we even have an iff: *)
-lemma isTrue_iff_prv_PPf: 
+(* In fact, by Minimal_Truth_Soundness we even have an iff: *)
+lemma isTrue_iff_bprv_PPf: 
 "\<And> n \<phi>. n \<in> num \<Longrightarrow> \<phi> \<in> fmla \<Longrightarrow> Fvars \<phi> = {} \<Longrightarrow> isTrue (PPf n \<langle>\<phi>\<rangle>) \<longleftrightarrow> bprv (PPf n \<langle>\<phi>\<rangle>)"
-using isTrue_implies_prv_PPf  
-using exists_no_Fvars not_isTrue_fls prv_sound_isTrue by auto
+using isTrue_implies_bprv_PPf  
+using exists_no_Fvars not_isTrue_fls bprv_sound_isTrue by auto
 
-(*  Truth of the provability representation implies provability: *)
-lemma isTrue_PP_implies_prv: 
+(*  Truth of the provability representation implies provability (TIP): *)
+lemma TIP: 
 assumes \<phi>[simp]: "\<phi> \<in> fmla" "Fvars \<phi> = {}"
 and iPP: "isTrue (wrepr.PP \<langle>\<phi>\<rangle>)"
 shows "prv \<phi>"
@@ -228,7 +229,7 @@ proof-
   have "isTrue (exi yy (PPf (Var yy) \<langle>\<phi>\<rangle>))" using iPP unfolding PP_PPf[OF \<phi>(1)] .
   from isTrue_exi[OF _ _ _ this] 
   obtain n where n[simp]: "n \<in> num" and "isTrue (PPf n \<langle>\<phi>\<rangle>)" by auto
-  hence pP: "bprv (PPf n \<langle>\<phi>\<rangle>)" using isTrue_implies_prv_PPf by auto
+  hence pP: "bprv (PPf n \<langle>\<phi>\<rangle>)" using isTrue_implies_bprv_PPf by auto
   hence "\<not> bprv (neg (PPf n \<langle>\<phi>\<rangle>))"  
   using prv_neg_excl[of "PPf n \<langle>\<phi>\<rangle>"] by auto 
   then obtain "prf" where "prf"[simp]: "prf \<in> proof" and nn: "n = encPf prf"  
@@ -242,7 +243,11 @@ thanks to our truth-in-standard-model assumption) *)
 
 
 lemmas HBL1_rev = \<omega>consistentStd1_HBL1_rev[OF B_\<omega>consistentStd1]
-(* Note: Would also follow by soundness from isTrue_PP_implies_prv *)
+(* Note: Would also follow by Minimal_Truth_Soundness from TIP:  *)
+lemma TIP_implies_HBL1_rev: 
+assumes TIP: "\<forall>\<phi>. \<phi> \<in> fmla \<and> Fvars \<phi> = {} \<and> isTrue (wrepr.PP \<langle>\<phi>\<rangle>) \<longrightarrow> prv \<phi>" 
+shows "\<forall>\<phi>. \<phi> \<in> fmla \<and> Fvars \<phi> = {} \<and> bprv (wrepr.PP \<langle>\<phi>\<rangle>) \<longrightarrow> prv \<phi>"
+using bprv_sound_isTrue[of "wrepr.PP \<langle>_\<rangle>"] TIP by auto
 
 end \<comment> \<open>Minimal_Truth_Soundness_Proof_Repr\<close>
 
@@ -328,9 +333,8 @@ lemma PPf_def2: "t1 \<in> trm \<Longrightarrow> t2 \<in> trm \<Longrightarrow> x
   unfolding PPf_def by (rule psubst_eq_rawpsubst2[simplified]) auto
 
 lemma Fvars_PPf[simp]: 
-"t1 \<in> trm \<Longrightarrow> t2 \<in> trm \<Longrightarrow> xx \<notin> FvarsT t1 \<Longrightarrow> 
- Fvars (PPf t1 t2) = FvarsT t1 \<union> FvarsT t2"
-by (auto simp add: PPf_def2 Fvars_subst subst2_fresh_switch)
+  "t1 \<in> trm \<Longrightarrow> t2 \<in> trm \<Longrightarrow> xx \<notin> FvarsT t1 \<Longrightarrow> Fvars (PPf t1 t2) = FvarsT t1 \<union> FvarsT t2"
+  by (auto simp add: PPf_def2 Fvars_subst subst2_fresh_switch)
 
 lemma [simp]: 
 "n \<in> num \<Longrightarrow> subst (PPf (Var yy) (Var xx)) n xx = PPf (Var yy) n"
@@ -348,19 +352,18 @@ lemma [simp]:
 lemma PP_PPf: 
 assumes "\<phi> \<in> fmla" "Fvars \<phi> = {}" shows "bprv (PP \<langle>\<phi>\<rangle>) \<longleftrightarrow> bprv (exi yy (PPf (Var yy) \<langle>\<phi>\<rangle>))"
   using assms PP_PPf_eqv[OF assms] B.prv_eqv_sym[OF _ _ PP_PPf_eqv[OF assms]]
-  apply safe apply(rule B.prv_eqv_prv[of "PP \<langle>\<phi>\<rangle>" "exi yy (PPf (Var yy) \<langle>\<phi>\<rangle>)"])
-  apply simp_all 
-  apply(rule B.prv_eqv_prv[of "exi yy (PPf (Var yy) \<langle>\<phi>\<rangle>)" "PP \<langle>\<phi>\<rangle>" ]) by auto
+  by (auto intro!: B.prv_eqv_prv[of "PP \<langle>\<phi>\<rangle>" "exi yy (PPf (Var yy) \<langle>\<phi>\<rangle>)"]
+    B.prv_eqv_prv[of "exi yy (PPf (Var yy) \<langle>\<phi>\<rangle>)" "PP \<langle>\<phi>\<rangle>"])
 
-lemma isTrue_implies_prv_PPf: 
+lemma isTrue_implies_bprv_PPf: 
 "\<And> n \<phi>. n \<in> num \<Longrightarrow> \<phi> \<in> fmla \<Longrightarrow> Fvars \<phi> = {} \<Longrightarrow>  
  isTrue (PPf n \<langle>\<phi>\<rangle>) \<Longrightarrow> bprv (PPf n \<langle>\<phi>\<rangle>)"
   using Compl_Pf by(simp add: PPf_def)
 
-lemma isTrue_iff_prv_PPf: 
+lemma isTrue_iff_bprv_PPf: 
 "\<And> n \<phi>. n \<in> num \<Longrightarrow> \<phi> \<in> fmla \<Longrightarrow> Fvars \<phi> = {} \<Longrightarrow> isTrue (PPf n \<langle>\<phi>\<rangle>) \<longleftrightarrow> bprv (PPf n \<langle>\<phi>\<rangle>)"
-using isTrue_implies_prv_PPf  
-  using exists_no_Fvars not_isTrue_fls prv_sound_isTrue by auto
+using isTrue_implies_bprv_PPf  
+  using exists_no_Fvars not_isTrue_fls bprv_sound_isTrue by auto
 
 
 
@@ -380,11 +383,11 @@ lemma prv_exi_PPf_iff_isTrue:
 assumes [simp]: "\<phi> \<in> fmla" "Fvars \<phi> = {}"  
 shows "bprv (exi yy (PPf (Var yy) \<langle>\<phi>\<rangle>)) \<longleftrightarrow> isTrue (exi yy (PPf (Var yy) \<langle>\<phi>\<rangle>))" (is "?L \<longleftrightarrow> ?R")
 proof
-  assume ?L thus ?R by (intro prv_sound_isTrue) auto
+  assume ?L thus ?R by (intro bprv_sound_isTrue) auto
 next
   assume ?R 
   obtain n where n[simp]: "n \<in> num" and i: "isTrue (PPf n \<langle>\<phi>\<rangle>)" using isTrue_exi[OF _ _ _ `?R`] by auto
-  hence "bprv (PPf n \<langle>\<phi>\<rangle>)" by (auto simp: isTrue_iff_prv_PPf)
+  hence "bprv (PPf n \<langle>\<phi>\<rangle>)" by (auto simp: isTrue_iff_bprv_PPf)
   thus ?L by (intro B.prv_exiI[of _ _ n]) auto
 qed
 
@@ -396,9 +399,9 @@ proof
 next
   assume ?R
   then obtain n where n[simp]: "n \<in> num" and i: "isTrue (PPf n \<langle>\<phi>\<rangle>)" by auto
-  hence "bprv (PPf n \<langle>\<phi>\<rangle>)" by (auto simp: isTrue_iff_prv_PPf)
+  hence "bprv (PPf n \<langle>\<phi>\<rangle>)" by (auto simp: isTrue_iff_bprv_PPf)
   hence "bprv (exi yy (PPf (Var yy) \<langle>\<phi>\<rangle>))" by (intro B.prv_exiI[of _ _ n]) auto
-  thus ?L by (intro prv_sound_isTrue) auto
+  thus ?L by (intro bprv_sound_isTrue) auto
 qed
 
 lemma prv_prfOf: 
@@ -409,7 +412,7 @@ proof-
   also have "\<dots> \<longleftrightarrow> bprv (exi yy (PPf (Var yy) \<langle>\<phi>\<rangle>))" unfolding PP_PPf[OF assms] ..
   also have "\<dots> \<longleftrightarrow> isTrue (exi yy (PPf (Var yy) \<langle>\<phi>\<rangle>))" using prv_exi_PPf_iff_isTrue[OF assms] .
   also have "\<dots> \<longleftrightarrow> (\<exists>n\<in>num. isTrue (PPf n \<langle>\<phi>\<rangle>))" using isTrue_exi_iff[OF assms] .
-  also have "\<dots> \<longleftrightarrow> (\<exists>n\<in>num. bprv (PPf n \<langle>\<phi>\<rangle>))" using isTrue_iff_prv_PPf[OF _ assms] by auto
+  also have "\<dots> \<longleftrightarrow> (\<exists>n\<in>num. bprv (PPf n \<langle>\<phi>\<rangle>))" using isTrue_iff_bprv_PPf[OF _ assms] by auto
   also have "\<dots> \<longleftrightarrow> (\<exists>n\<in>num. prfOf n \<phi>)" unfolding prfOf_def ..
   finally show ?thesis .
 qed 
@@ -428,10 +431,28 @@ proof-
   hence "bprv (imp (PP \<langle>\<phi>\<rangle>) (exi yy (PPf (Var yy) \<langle>\<phi>\<rangle>)))"
   and "bprv (imp (exi yy (PPf (Var yy) \<langle>\<phi>\<rangle>)) (PP \<langle>\<phi>\<rangle>))"  
   by (simp_all add: B.prv_imp_eqvEL B.prv_imp_eqvER)   
-  thus ?thesis unfolding isTrue_exi_iff[OF assms, symmetric] 
-  apply safe apply(rule prv_imp_implies_isTrue) apply simp_all
-  apply(rule prv_imp_implies_isTrue) by simp_all
+  thus ?thesis unfolding isTrue_exi_iff[OF assms, symmetric]
+    by (intro iffI) (rule prv_imp_implies_isTrue; simp)+
 qed
+
+lemma bprv_compl_isTrue_PP_enc: 
+assumes 1: "\<phi> \<in> fmla" "Fvars \<phi> = {}" and 2: "isTrue (PP \<langle>\<phi>\<rangle>)"
+shows "bprv (PP \<langle>\<phi>\<rangle>)"
+proof-
+  obtain n where nn: "n \<in> num" and i: "isTrue (PPf n \<langle>\<phi>\<rangle>)" 
+   using 2 unfolding isTrue_exi_iff_PP[OF 1] .. 
+  hence "bprv (PPf n \<langle>\<phi>\<rangle>)" 
+    using i using nn assms isTrue_iff_bprv_PPf by blast
+  hence "bprv (exi yy (PPf (Var yy) \<langle>\<phi>\<rangle>))"  
+  using 2 assms isTrue_exi_iff isTrue_exi_iff_PP prv_exi_PPf_iff_isTrue by auto
+  thus ?thesis using PP_PPf 1 by blast
+qed 
+
+lemma TIP: 
+assumes 1: "\<phi> \<in> fmla" "Fvars \<phi> = {}" and 2: "isTrue (PP \<langle>\<phi>\<rangle>)"
+shows "prv \<phi>"
+using bprv_compl_isTrue_PP_enc[OF assms] HBL1_iff assms by blast
+ 
 
 end \<comment> \<open>context Minimal_Truth_Soundness_HBL1iff_Compl_Pf\<close>
 
@@ -454,14 +475,14 @@ lemma isTrue_implies_prv_neg_PPf:
 lemma isTrue_iff_prv_neg_PPf: 
 "\<And> n \<phi>. n \<in> num \<Longrightarrow> \<phi> \<in> fmla \<Longrightarrow> Fvars \<phi> = {} \<Longrightarrow> isTrue (neg (PPf n \<langle>\<phi>\<rangle>)) \<longleftrightarrow> bprv (neg (PPf n \<langle>\<phi>\<rangle>))"
 using isTrue_implies_prv_neg_PPf  
-  using exists_no_Fvars not_isTrue_fls prv_sound_isTrue by auto
+  using exists_no_Fvars not_isTrue_fls bprv_sound_isTrue by auto
 
 lemma prv_PPf_decide: 
 assumes [simp]: "n \<in> num" "\<phi> \<in> fmla" "Fvars \<phi> = {}"
 and np: "\<not> bprv (PPf n \<langle>\<phi>\<rangle>)"
 shows "bprv (neg (PPf n \<langle>\<phi>\<rangle>))"
 proof-
-  have "\<not> isTrue (PPf n \<langle>\<phi>\<rangle>)" using assms by (auto simp: isTrue_iff_prv_PPf)
+  have "\<not> isTrue (PPf n \<langle>\<phi>\<rangle>)" using assms by (auto simp: isTrue_iff_bprv_PPf)
   hence "isTrue (neg (PPf n \<langle>\<phi>\<rangle>))" using isTrue_neg[of "PPf n \<langle>\<phi>\<rangle>"] by auto
   thus ?thesis by (auto simp: isTrue_iff_prv_neg_PPf)
 qed 
@@ -480,16 +501,13 @@ in Minimal_Truth_Soundness_HBL1iff_Compl_Pf but defined in Repr_Proofs
 (they are of course extensionally equal).
 *)
   where "proof" = "proof" and prfOf = prfOf and encPf = encPf  
-  apply standard
-  apply (auto simp: bprv_prv prv_prfOf prfOf_prv_Pf not_prfOf_prv_neg_Pf)
-  done
+  by standard (auto simp: bprv_prv prv_prfOf prfOf_prv_Pf not_prfOf_prv_neg_Pf)
 
 (* Lemma 6 ("proof recovery") from the JAR paper: *)
 sublocale Minimal_Truth_Soundness_HBL1iff_Compl_Pf_Compl_NegPf < 
   min_truth: Minimal_Truth_Soundness_Proof_Repr
 where "proof" = "proof" and prfOf = prfOf and encPf = encPf
-  apply standard 
-  done
+  by standard
 
 
 
@@ -499,14 +517,14 @@ locale Minimal_Truth_Soundness_HBL1iff_prv_Compl_Pf =
 WRepr_Provability
   var trm fmla Var FvarsT substT Fvars subst
   num
-  eql cnj imp all exi 
+  eql cnj imp all exi
   prv bprv 
   enc 
   P
 +
 Minimal_Truth_Soundness
   var trm fmla Var FvarsT substT Fvars subst
-  eql cnj imp all exi 
+  eql cnj imp all exi
   fls
   dsj
   num
@@ -564,17 +582,14 @@ lemma HBL1_iff: "\<phi> \<in> fmla \<Longrightarrow> Fvars \<phi> = {} \<Longrig
   using HBL1 HBL1_rev unfolding PP_def by auto
 
 lemma HBL1_iff_prv: "\<phi> \<in> fmla \<Longrightarrow> Fvars \<phi> = {} \<Longrightarrow> prv (PP \<langle>\<phi>\<rangle>) \<longleftrightarrow> prv \<phi>"
-  apply safe
-  using HBL1_rev_prv apply simp
-  using bprv_prv HBL1_PP by auto 
+  by (intro iffI bprv_prv[OF _ _ HBL1_PP], elim HBL1_rev_prv[rotated -1]) auto
 
 end (* context Minimal_Truth_Soundness_HBL1iff_prv_Compl_Pf *)
 
 sublocale Minimal_Truth_Soundness_HBL1iff_prv_Compl_Pf < 
-mts_prv_mts: Minimal_Truth_Soundness_HBL1iff_Compl_Pf where Pf = Pf
-  apply standard  
-  using P_Pf HBL1_rev HBL1_PP Compl_Pf by auto
-
+  mts_prv_mts: Minimal_Truth_Soundness_HBL1iff_Compl_Pf where Pf = Pf
+  using P_Pf HBL1_rev HBL1_PP Compl_Pf
+  by unfold_locales auto
 
 locale Minimal_Truth_Soundness_HBL1iff_prv_Compl_Pf_Classical = 
 Minimal_Truth_Soundness_HBL1iff_prv_Compl_Pf
@@ -595,6 +610,5 @@ end \<comment> \<open>context Minimal_Truth_Soundness_HBL1iff_Compl_Pf_Variant_C
 
 
   
-
 
 end 
