README.md
@@ -1,13 +1,9 @@
-This repository contains the Isabelle formalization of abstract formulations
-of Gödel's Incompleteness Theorems related to the article
+This repository contains the Isabelle formalization of abstract formulations of Gödel's Incompleteness Theorems related to the paper
 
-> **Distilling the Requirements of Gödel's Incompleteness Theorems with a Proof Assistant**
->
-> Andrei Popescu, Dmitriy Traytel
+**Distilling the Requirements of Gödel’s Incompleteness Theorems with a Proof Assistant**
+by Andrei Popescu and Dmitriy Traytel
 
-The formal development can be browsed as a generated HTML page
-(see the ```html``` directory). A better way to study the theory files, however, is to open
-them in Isabelle/jEdit.
+The formal development can be browsed as a generated HTML page (see the ```html``` directory). A better way to study the theory files, however, is to open them in Isabelle/jEdit.
 
 The raw Isabelle sources are included in a separate directory called ```thys```.
 
@@ -27,20 +23,13 @@ processed. With Isabelle up and running it should take only 5 minutes.
 
 ### Organization
 
-The formalization of the abstract theory and the concrete instances is organized in four sessions
-(see ROOT file):
+The formalization of the abstract theory and the concrete instances is organized in four sessions (see ROOT file):
 
-1. ```Abstract```: contains all our abstract infrastructure and results (from paper's Sections 2 and 3).
+1. ```Abstract```: contains all our abstract infrastructure and results (from paper's Sections 4--8).
 
-2. ```HF_Sets_Semantic_First_and_Second```: contains the instantiation of our abstract infrastructure with Paulson's
-notions stemming from his formalization of the First and Second Incompleteness theorems (from the AFP entry
-Incompleteness), including the soundness assumption for the underlying theory. The instantiation
-results in a reproduction of Paulson's First and Second Incompleteness theorem.
+2. ```HF_Sets_Semantic_First_and_Second```: contains the instantiation of our abstract infrastructure with Paulson's notions stemming from his formalization of the First and Second Incompleteness theorems (from the AFP entry Incompleteness), including the soundness assumption for the underlying theory. The instantiation results in a reproduction of Paulson's First and Second Incompleteness theorem.
 
-3. ```HF_Sets_Semanticless_Second```: contains the instantiation of our abstract infrastructure with an improved version
-of Paulson's notions, which this time do *not* assume soundness of the underlying calculus. The instantiation
-results in an upgrade of Paulson's Second Incompleteness theorem, which now supports consistent, but not
-necessarily sound theory. To achieve this we have adjusted some of Paulson's theories, which are contained in ```thys/Incompleteness```.
+3. ```HF_Sets_Semanticless_Second```: contains the instantiation of our abstract infrastructure with an improved version of Paulson's notions, which this time do *not* assume soundness of the underlying calculus. The instantiation results in an upgrade of Paulson's Second Incompleteness theorem, which now supports consistent, but not necessarily sound theory. To achieve this we have adjusted some of Paulson's theories, which are contained in ```thys/Incompleteness```.
 
 4. ```Robinson_Arith```: contains the instantiation of the logic and arithmetic part of our abstract infrastructure
 with the syntax and semantics of the Robinson Arithmetic (System Q).
@@ -51,113 +40,107 @@ To process them, Isabelle must be invoked as follows:
 
 ```isabelle jedit -d '<path/to/afp>/thys' -d 'thys'```
 
-where the first path points to the ```thys``` directory in the AFP installation
-and the second points to the ```thys``` directory of this repository.
+where the first path points to the ```thys``` directory in the AFP installation and the second points to the ```thys``` directory of this repository.
 
-Acknowledgement: As noted in the paper, our instantiation to hereditarily finite sets uses
-many lemmas proved by Larry Paulson. Our instantiation to System Q also adapts to the new syntax many of
-Paulson's constructions and proofs using Nominal Isabelle.
+Acknowledgement: As noted in the paper, our instantiation to hereditarily finite sets uses many lemmas proved by Larry Paulson. Our instantiation to System Q also adapts to the new syntax many of Paulson's constructions and proofs using Nominal Isabelle.
 
 
 ### Isabelle Specifics
 
-The reader should be able to easily recognize in our formal scripts the concepts and results
-reported in the paper -- based on the aforementioned separation into sessions and guided by the
-theories' self-explanatory names. Moreover, the scripts use notations similar to the paper,
-with minor variations, e.g., "fmla" instead of "Fmla". (Some notation variations are pointed out
-below.)
+The reader should be able to easily recognize in our formal scripts the concepts and results reported in the paper -- based on the aforementioned separation into sessions and guided by the theories' self-explanatory names. Moreover, the scripts use notations similar to the paper, with minor variations, e.g., "fmla" instead of "Fmla". (Some notation variations are pointed out below.)
 
 Next we list some points of difference:
 
-1) To better manage the many assumptions, the formal theorems are organized into Isabelle locales,
-again having self-explanatory names: for example, the locale ```Deduct_with_PseudoOrder```
-puts together logical deduction and the order-like relation. Consequently,
-to identify a theorem's assumptions we need to look at both its explicit assumptions and
-its underlying locale's assumptions: for example, the theorem ```godel_rosser_first``` has
-only one explicit assumption (consistency), but more assumptions coming from its locale ```Rosser_Form```.
+1) To better manage the many assumptions, the formal theorems are organized into Isabelle locales, again having self-explanatory names: For example, the locale ```Deduct_with_PseudoOrder``` puts together logical deduction and the order-like relation. Consequently, to identify a theorem's assumptions we need to look at both its explicit assumptions and its underlying locale's assumptions: for example, the theorem ```godel_rosser_first``` has only one explicit assumption (consistency), but more assumptions coming from its locale ```Rosser_Form```.
 
 Information about locales can be found at
 [https://isabelle.in.tum.de/website-Isabelle2020-RC3/dist/Isabelle2020-RC3/doc/locales.pdf](https://isabelle.in.tum.de/website-Isabelle2020-RC3/dist/Isabelle2020-RC3/doc/locales.pdf)
 
+2) The formal scripts are obviously much more detailed than the proof sketches shown in the paper, and contain significantly more lemmas. In particular, for our logical infrastructure (theories ```Deduction``` and ```Natural_Deduction```) we have proved a very large amounts of facts, significantly more than we needed for the current theorems. This was done while keeping in mind our longer-term goal of instantiating our results more broadly, where a well developed logical infrastructure will help.
 
-2) The formal scripts are obviously much more detailed than the
-proof sketches shown in the paper and in the appendix, and contain significantly more lemmas.
-In particular, for our logical infrastructure (theories ```Deduction``` and ```Natural_Deduction```)
-we have proved a very large amounts of facts, significantly more than we needed for the current
-theorems. This was done while keeping in mind our longer-term goal of instantiating our results more
-broadly, where a well developed logical infrastructure will help.
-
-3) For the same reason (ease of future instantiation), our various types of entities (terms, numerals,
-formulas, proofs, etc.) do not form entire Isabelle types, but rather subsets of types: For example,
-formulas are a set "fmla" of type "'fmla set" rather than the whole type 'fmla.
+3) For the same reason (ease of future instantiation), our various types of entities (terms, numerals, formulas, proofs, etc.) do not form entire Isabelle types, but rather subsets of types: For example, formulas are a set "fmla" of type "'fmla set" rather than the whole type 'fmla.
 
 4) We use curried operators rather than operators on product types.
 
-5) In addition to Goedel's incompleteness theorems, our abstract development includes the
-very related theorems of Loeb and Tarski. The latter did not make it into the paper.
+5) In addition to Gödel's incompleteness theorems, our abstract development includes the very related theorems of Löb and Tarski. The latter did not make it into the paper.
 
-6) On few occasions, we use different but quite self-explanatory notations: "prv", "pprv" and
-"isTrue" for the provability, "proof of" and truth predicates; "P" and "Pf" for the representations
-of "prv", "pprv"; "N" and "S" for the representations of negation and self-substitution.
-We also use "double" notation for the Isabelle functions that instantiate the representation formulas
-to different terms: e.g., "PP t" denotes what in the paper we would write "P(t)", namely the
-formula obtained from P by substituting its single variable with the term t.
+6) On few occasions, we use different but quite self-explanatory notations: "prv", "pprv" and "isTrue" for the provability, "proof of" and truth predicates; "P" and "Pf" for the representations of "prv", "pprv"; "N" and "S" for the representations of negation and self-substitution. We write "bprv" for basic provability. We also use "double" notation for the Isabelle functions that instantiate the representation formulas to different terms: e.g., "PP t" denotes what in the paper we would write "P(t)", namely the formula obtained from P by substituting its single variable with the term t.
 
-7) Here is how the paper's theorems can be found in the formal scripts. Each time, we show the formal
-theorem's name (or refer to some locale instantiations) and the containing Isabelle theory.
+7) Here is how the paper's theorems can be found in the formal scripts. Each time, we show the formal theorem's name (or refer to some locale instantiations) and the containing Isabelle theory.
 
-Lemma 3:
+Lemma 4 => ```HBL1``` from theory ```Abstract_Representability```.
+
+Lemma 6:
 (1) => ```ωconsistentStd1_HBL1_rev``` from theory ```Abstract_Representability```;
-(2) => ```ωconsistent``` from theory ```Abstract_Models```;
-(3) => ```isTrue_PP_implies_prv``` from theory ```Abstract_Model```
+(2)  =>  ```TIP_implies_HBL1_rev``` from theory ```Abstract_Model```
+(3) => ```TIP``` from theory ```Abstract_Model```
 
-Lamma 4 => ```prv_prfOf```, ```prfOf_prv_Pf``` and ```not_prfOf_prv_neg_Pf```
-from theory ```Standard_Models```
+Lamma 7 => ```prv_prfOf```, ```prfOf_prv_Pf``` and ```not_prfOf_prv_neg_Pf``` from theory ```Standard_Model```
 
-Prop 5 => diagonalization from Diagonalizaton
+Lemma 8:
+(1) =>   ```bprv_compl_isTrue_PP_enc```  from theory ```Standard_Model```
+(2) =>  ```TIP ``` from theory ```Standard_Model```
 
-Prop 6:
-Goedel sentence => ```prv_φG_eqv``` from ```Godel_Formula```;
-Rosser sentence => ```prv_φR_eqv``` from ```Rosser_Formula```
+Prop 9 => ```diagonalization```  from theory Diagonalizaton
 
-Prop 7 => ```godel_first_theEasyHalf``` from ```Abstract_First_Godel```
+Prop 10:
+(Basic) Gödel sentence => ```bprv_φG_eqv``` and ```prv_φG_eqv``` from theory ```Godel_Formula```;
+(Basic) Rosser sentence => ```bprv_φR_eqv``` and ```prv_φR_eqv```  from theory ```Rosser_Formula```
 
-Prop 8 => ```godel_first_theHardHalf``` from ```Abstract_First_Godel```
+Prop 11 => ```godel_first_theEasyHalf``` from theory ```Abstract_First_Godel```
 
-Theorem 9 => ```godel_first``` from ```Abstract_First_Godel```
+Prop 12 => ```godel_first_theHardHalf``` from theory ```Abstract_First_Godel```
 
-Theorem 10 => ```godel_rosser_first``` from ```Abstract_First_Godel_Rosser```
+Theorem 13 => ```godel_first``` from theory ```Abstract_First_Godel```
 
-Theorem 11 => ```godel_first_strong``` from ```Abstract_First_Godel```
+Prop 14 =>  ```godel_rosser_first_theHardHalf``` from theory ```Abstract_First_Godel_Rosser```
 
-Theorem 12 => ```godel_first_classic``` from ```Abstract_First_Godel```
+Prop 15 =>  ```godel_rosser_first_theEasyHalf``` from theory ```Abstract_First_Godel_Rosser```
 
-Theorem 13 => godel_second from ```Abstract_Second_Godel```
+Theorem 16 => ```godel_rosser_first``` from theory ```Abstract_First_Godel_Rosser```
 
-Lemma 15 => diagonalization from Jeroslow
+Theorem 17 => ```godel_first_strong``` from theory ```Abstract_First_Godel```
 
-Theorem 16 => ```jeroslow_godel_second``` from Jeroslow
+Theorem 18 => ```recover_proofs.godel_first_strong``` from theory ```Abstract_First_Godel```
 
-Theorem 17 => ```jeroslow_godel_second_modified``` from Jeroslow
+Theorem 19 => ```godel_rosser_first_strong``` from theory ```Abstract_First_Godel```
 
-Prop 18:
+Theorem 20 => ```recover_proofs.godel_rosser_first_strong``` from theory ```Abstract_First_Godel```
+
+Lemma 21 => ```B_ωconsistent``` from theory ```Standard_Model```
+
+Theorem 22 => ```godel_first_classic``` from theory ```Abstract_First_Godel```
+
+Theorem 23 => ```godel_first_classic_strong``` from theory ```Abstract_First_Godel```
+
+Theorem 24 => ```recover_proofs.godel_first_classic_strong``` from theory ```Abstract_First_Godel```
+
+Theorem 25 => ```godel_second from```  from theory ```Abstract_Second_Godel```
+
+Example 28:
+(1) => ```prveqlPT_prv_instInp_eqv_cmpP```  from theory ```PseudoTerms```
+(2) => ```prv_cmpP_compose```  from theory ```PseudoTerms```
+
+Lemma 29 =>  ```diagonalization```  from theories
+```Jeroslow``` and ```Jeroslow_Corrected```
+
+Theorem 30 => ```jeroslow_godel_second```  from theories
+```Jeroslow``` and ```Jeroslow_Corrected```
+
+Prop 31 =>  ```jcons_implies_neg_PP_fls```  from theory  ```Jeroslow_Corrected```
+
+Theorem 32 => ```jeroslow_godel_second_standardCon```  from theory  ```Jeroslow_Corrected```
+
+Prop 33:
 (1) => The locale instantiations from theories
 ```Q_Instance_Syntax_Deduction```, ```Q_Instance_Theory```;
 and part of the locale instantiations from theory ```HF_Instance```;
 (2) => The locale instantiations from theory```Q_Instance_Sound```;
 and part of the locale instantiations from theory ```HF_Instance_Weak```
 
-Theorem 19:
+Theorem 34:
 (1) => the locale instantiations from theory ```HF_Instance_Weak```;
 (2) => the locale instantiations from theory ```HF_Instance```
-
-
-
-
-
-
-
-
 
 
 
